Puar/WordFacts.v
@@ -1,0 +1,255 @@
+(*! TODO: merge with Word.v !*)
+
+Require Import ZArith Eqdep.
+Require Import Lib.CommonTactics Lib.NatLib Lib.Word.
+
+Set Implicit Arguments.
+
+(* some more manipulation on [word] *)
+
+Definition extz {sz} (w: word sz) (n: nat) := combine (wzero n) w.
+
+Definition rtrunc1 sz (w: word (S sz)): word sz:=
+  match w with
+  | WO => idProp
+  | WS _ w' => w'
+  end.
+
+Definition rtrunc2 sz (w: word (S (S sz))): word sz :=
+  match w with
+  | WO => idProp
+  | WS _ w' =>
+    match w' with
+    | WO => idProp
+    | WS _ w'' => w''
+    end
+  end.
+
+Definition wlsb sz (w: word (S sz)) :=
+  match w with
+  | WO => idProp
+  | WS b _ => b
+  end.
+
+(* some more facts *)
+
+Lemma wordToZ_wzero':
+  forall sz, wordToZ (wzero' sz) = 0%Z.
+Proof.
+Admitted.
+
+Lemma combine_wplus:
+  forall sl (w1: word sl) su (w2 w3: word su),
+    combine w1 (w2 ^+ w3) = combine w1 w2 ^+ extz w3 sl.
+Proof.
+Admitted.
+
+Lemma existT_wplus:
+  forall sz (w1 w2: word sz) sz' (w3 w4: word sz'),
+    existT word _ w1 = existT word _ w3 ->
+    existT word _ w2 = existT word _ w4 ->
+    existT word _ (w1 ^+ w2) = existT word _ (w3 ^+ w4).
+Proof.
+  intros.
+  rewrite eq_sigT_sig_eq in H; destruct H as [Hsz1 ?].
+  rewrite eq_sigT_sig_eq in H0; destruct H0 as [Hsz2 ?].
+  subst; do 2 rewrite <-eq_rect_eq.
+  reflexivity.
+Qed.
+
+Lemma wrshifta_wplus:
+  forall sz (w1 w2: word sz) n,
+    wrshifta (w1 ^+ w2) n = wrshifta w1 n ^+ wrshifta w2 n.
+Proof.
+Admitted.
+
+Lemma combine_wrshifta_rtrunc1_sext:
+  forall s (w: word s) sl (wl: word (S (S sl))) su (wu: word su),
+    existT word s w =
+    existT word ((S (S sl)) + su) (combine wl wu) ->
+    existT word s (wrshifta w 1) =
+    existT word ((S sl) + (su + 1)) (combine (rtrunc1 wl) (sext wu 1)).
+Proof.
+Admitted.
+
+Lemma combine_wrshifta_rtrunc2_sext:
+  forall s (w: word s) sl (wl: word (S (S (S sl)))) su (wu: word su),
+    existT word s w =
+    existT word ((S (S (S sl))) + su) (combine wl wu) ->
+    existT word s (wrshifta w 2) =
+    existT word ((S sl) + (su + 2)) (combine (rtrunc2 wl) (sext wu 2)).
+Proof.
+Admitted.
+
+Lemma wrshifta_extz_sext:
+  forall sz (w: word sz) n1 n2,
+    existT word _ (wrshifta (extz w (n1 + n2)) n1) =
+    existT word _ (sext (extz w n2) n1).
+Proof.
+Admitted.
+
+Lemma wlshift_sext_extz:
+  forall sz (w: word sz) n,
+    existT word _ (wlshift (sext w n) n) =
+    existT word _ (extz w n).
+Proof.
+Admitted.
+
+Lemma extz_sext:
+  forall sz (w: word sz) n1 n2,
+    existT word _ (extz (sext w n1) n2) =
+    existT word _ (sext (extz w n2) n1).
+Proof.
+Admitted.
+
+Lemma extz_sext_eq_rect:
+  forall sz (w: word sz) n1 n2 nsz Hnsz1,
+  exists Hnsz2,
+    eq_rect (n2 + (sz + n1)) word (extz (sext w n1) n2) nsz Hnsz1 =
+    eq_rect (n2 + sz + n1) word (sext (extz w n2) n1) nsz Hnsz2.
+Proof.
+  intros; subst; simpl.
+  assert (Hsz: n2 + sz + n1 = n2 + (sz + n1)) by omega.
+  exists Hsz.
+  pose proof (extz_sext w n1 n2).
+  pose proof (eq_sigT_snd H).
+  rewrite <-H0.
+  eq_rect_simpl.
+  reflexivity.
+Qed.
+
+Lemma existT_sext:
+  forall sz1 (w1: word sz1) sz2 (w2: word sz2) n,
+    existT word _ w1 = existT word _ w2 ->
+    existT word _ (sext w1 n) = existT word _ (sext w2 n).
+Proof.
+  intros; inv H; reflexivity.
+Qed.
+
+Lemma existT_extz:
+  forall sz1 (w1: word sz1) sz2 (w2: word sz2) n,
+    existT word _ w1 = existT word _ w2 ->
+    existT word _ (extz w1 n) = existT word _ (extz w2 n).
+Proof.
+  intros; inv H; reflexivity.
+Qed.
+
+Lemma existT_wrshifta:
+  forall sz1 (w1: word sz1) sz2 (w2: word sz2) n,
+    existT word _ w1 = existT word _ w2 ->
+    existT word _ (wrshifta w1 n) = existT word _ (wrshifta w2 n).
+Proof.
+  intros; inv H; reflexivity.
+Qed.
+
+Lemma existT_wlshift:
+  forall sz1 (w1: word sz1) sz2 (w2: word sz2) n,
+    existT word _ w1 = existT word _ w2 ->
+    existT word _ (wlshift w1 n) = existT word _ (wlshift w2 n).
+Proof.
+  intros; inv H; reflexivity.
+Qed.
+
+Lemma extz_extz:
+  forall sz (w: word sz) n1 n2,
+    existT word _ (extz (extz w n1) n2) =
+    existT word _ (extz w (n2 + n1)).
+Proof.
+Admitted.
+
+Lemma sext_wplus_wordToZ_distr:
+  forall sz (w1 w2: word sz) n,
+    n <> 0 -> wordToZ (sext w1 n ^+ sext w2 n) =
+              (wordToZ (sext w1 n) + wordToZ (sext w2 n))%Z.
+Proof.
+Admitted.
+
+Lemma sext_wordToZ:
+  forall sz (w: word sz) n,
+    wordToZ (sext w n) = wordToZ w.
+Proof.
+Admitted.
+
+Lemma split1_combine_existT:
+  forall sz n (w: word (n + sz)) sl (wl: word (n + sl)) su (wu: word su),
+    existT word _ w = existT word _ (combine wl wu) ->
+    split1 n _ w = split1 n _ wl.
+Proof.
+Admitted.
+
+Lemma extz_pow2_wordToZ:
+  forall sz (w: word sz) n,
+    wordToZ (extz w n) = (wordToZ w * Z.of_nat (pow2 n))%Z.
+Proof.
+Admitted.
+
+Lemma extz_wneg:
+  forall sz (w: word sz) n,
+    extz (wneg w) n = wneg (extz w n).
+Proof.
+Admitted.
+
+Lemma wneg_wordToZ:
+  forall sz (w: word sz),
+    wordToZ (wneg w) = (- wordToZ w)%Z.
+Proof.
+Admitted.
+
+Lemma wneg_wordToZ':
+  forall sz (w: word sz) z,
+    (z + wordToZ (wneg w))%Z = (z - wordToZ w)%Z.
+Proof.
+  intros; rewrite wneg_wordToZ; omega.
+Qed.
+
+Lemma wrshifta_zero:
+  forall sz n, wrshifta (natToWord sz 0) n = wzero _.
+Proof.
+Admitted.
+
+Lemma extz_zero:
+  forall sz n, extz (natToWord sz 0) n = wzero _.
+Proof.
+Admitted.
+
+Lemma existT_eq_rect:
+  forall (X: Type) (P: X -> Type) (x1 x2: X) (H1: P x1) (Hx: x1 = x2),
+    existT P x2 (eq_rect x1 P H1 x2 Hx) =
+    existT P x1 H1.
+Proof.
+  intros; subst.
+  rewrite <-eq_rect_eq; reflexivity.
+Qed.
+
+Lemma sext_eq_rect:
+  forall sz (w: word sz) n nsz Hsz1,
+  exists Hsz2,
+    eq_rect (sz + n) word (sext w n) (nsz + n) Hsz1 =
+    sext (eq_rect sz word w nsz Hsz2) n.
+Proof.
+  intros.
+  assert (Hsz: sz = nsz) by omega.
+  exists Hsz.
+  subst; simpl.
+  eq_rect_simpl.
+  reflexivity.
+Qed.
+
+Lemma wordToZ_eq_rect:
+  forall sz (w: word sz) nsz Hsz,
+    wordToZ (eq_rect _ word w nsz Hsz) = wordToZ w.
+Proof.
+  intros; subst; simpl; reflexivity.
+Qed.
+
+Lemma pow2_S_z:
+  forall n, Z.of_nat (pow2 (S n)) = (2 * Z.of_nat (pow2 n))%Z.
+Proof.
+  intros.
+  replace (2 * Z.of_nat (pow2 n))%Z with
+      (Z.of_nat (pow2 n) + Z.of_nat (pow2 n))%Z by omega.
+  simpl.
+  repeat rewrite Nat2Z.inj_add.
+  ring.
+Qed.
+
